More FCtx work

FreydSSA/FCtx.lean
@@ -15,7 +15,7 @@ structure FCtx (ν : Type u) (α : Type v) : Type (max u v) where
   support : Finset ν
   mem_support_toFun : ∀x, x ∈ support ↔ toFun x ≠ ⊥
 
-theorem FCtx.ext {Γ Δ : FCtx ν α} (h : Γ.toFun = Δ.toFun)
+theorem FCtx.toFun_inj_mp {Γ Δ : FCtx ν α} (h : Γ.toFun = Δ.toFun)
   : Γ = Δ
   := match Γ, Δ with
   | ⟨fΓ, n, hm⟩, ⟨fΔ, n', hm'⟩ => by
@@ -25,13 +25,46 @@ theorem FCtx.ext {Γ Δ : FCtx ν α} (h : Γ.toFun = Δ.toFun)
     intro x
     rw [hm, hm']
 
-theorem FCtx.ext_iff {Γ Δ : FCtx ν α}
+theorem FCtx.toFun_inj {Γ Δ : FCtx ν α}
   : Γ = Δ ↔ Γ.toFun = Δ.toFun
-  := ⟨(λh => by cases h; rfl), FCtx.ext⟩
+  := ⟨(λh => by cases h; rfl), FCtx.toFun_inj_mp⟩
+
+--TODO: Injective instance? Naming convention...
 
 instance FCtx.instFunLike : FunLike (FCtx ν α) ν (WithBot α) where
   coe := FCtx.toFun
-  coe_injective' := by intro Γ Δ; apply FCtx.ext
+  coe_injective' := by intro Γ Δ; apply FCtx.toFun_inj_mp
+
+theorem FCtx.ext {Γ Δ : FCtx ν α} (h : ∀x, Γ x = Δ x)
+  : Γ = Δ
+  := DFunLike.coe_injective' (by funext x; apply h)
+
+theorem FCtx.mem_support {Γ : FCtx ν α} (x : ν)
+  : x ∈ Γ.support ↔ Γ x ≠ ⊥ := Γ.mem_support_toFun x
+
+theorem FCtx.mem_support_exists {Γ : FCtx ν α} (x : ν)
+  : x ∈ Γ.support ↔ ∃a : α, Γ x = a := by
+  rw [mem_support]
+  apply Iff.intro
+  . cases Γ x with
+    | none => intro h; contradiction
+    | some a => intro _; exact ⟨a, rfl⟩
+  . intro ⟨a, ha⟩
+    rw [ha]
+    simp
+
+theorem FCtx.mem_support_of_var {Γ : FCtx ν α} (x : ν) (a : α)
+  (h : Γ x = a) : x ∈ Γ.support := by
+  rw [mem_support]
+  intro h'
+  rw [h] at h'
+  contradiction
+
+theorem FCtx.not_mem_support_of_null {Γ : FCtx ν α} (x : ν)
+  (h : Γ x = ⊥) : x ∉ Γ.support := by
+  rw [mem_support]
+  intro h'
+  contradiction
 
 def FCtx.map_ty (Γ : FCtx ν α) (f : α → β) : FCtx ν β where
   toFun x := (Γ.toFun x).map (f)
@@ -57,7 +90,7 @@ def FCtx.cons_inj {x : ν} {a a' : α} {Γ : FCtx ν α}
   have hr : Γ.cons x a' x = a' := by simp [FCtx.cons, DFunLike.coe]
   by rw [<-WithBot.coe_inj, <-hl, <-hr, h]
 
-def FCtx.Wk (Γ Δ : FCtx ν α) : Prop := ∀x, Δ.toFun x = ⊥ ∨ Δ.toFun x = Γ.toFun x
+def FCtx.Wk (Γ Δ : FCtx ν α) : Prop := ∀x, Δ x = ⊥ ∨ Δ x = Γ x
 
 theorem FCtx.Wk.refl (Γ : FCtx ν α) : FCtx.Wk Γ Γ := by simp [FCtx.Wk]
 theorem FCtx.Wk.trans {Γ Δ Θ : FCtx ν α} (w : FCtx.Wk Γ Δ) (w' : FCtx.Wk Δ Θ)
@@ -67,7 +100,7 @@ theorem FCtx.Wk.trans {Γ Δ Θ : FCtx ν α} (w : FCtx.Wk Γ Δ) (w' : FCtx.Wk 
 theorem FCtx.Wk.antisymm {Γ Δ : FCtx ν α} (w : FCtx.Wk Γ Δ) (w' : FCtx.Wk Δ Γ)
   : Γ = Δ := by
   apply FCtx.ext
-  funext x
+  intro x
   cases w x with
   | inl h => cases w' x with | inl h' => rw [h, h'] | inr h' => exact h'
   | inr h => exact h.symm
@@ -75,13 +108,13 @@ theorem FCtx.Wk.antisymm {Γ Δ : FCtx ν α} (w : FCtx.Wk Γ Δ) (w' : FCtx.Wk 
 def FCtx.Wk.src {Γ Δ : FCtx ν α} (_ : FCtx.Wk Γ Δ) : FCtx ν α := Γ
 def FCtx.Wk.trg {Γ Δ : FCtx ν α} (_ : FCtx.Wk Γ Δ) : FCtx ν α := Δ
 
-theorem FCtx.Wk.eq_bot {Γ Δ : FCtx ν α} (w : FCtx.Wk Γ Δ) (x : ν) (h : Γ.toFun x = ⊥)
-  : Δ.toFun x = ⊥ := by cases w x <;> simp [*]
-theorem FCtx.Wk.ne_bot {Γ Δ : FCtx ν α} (w : FCtx.Wk Γ Δ) (x : ν) (h : Δ.toFun x ≠ ⊥)
-  : Γ.toFun x ≠ ⊥ := λh' => h (w.eq_bot _ h')
+theorem FCtx.Wk.eq_bot {Γ Δ : FCtx ν α} (w : FCtx.Wk Γ Δ) (x : ν) (h : Γ x = ⊥)
+  : Δ x = ⊥ := by cases w x <;> simp [*]
+theorem FCtx.Wk.ne_bot {Γ Δ : FCtx ν α} (w : FCtx.Wk Γ Δ) (x : ν) (h : Δ x ≠ ⊥)
+  : Γ x ≠ ⊥ := λh' => h (w.eq_bot _ h')
 theorem FCtx.Wk.eq_some_ne_bot {Γ Δ : FCtx ν α} (w : FCtx.Wk Γ Δ)
-  (x : ν) (h : Δ.toFun x ≠ ⊥)
-  : Γ.toFun x ≠ ⊥ := λh' => h (w.eq_bot _ h')
+  (x : ν) (h : Δ x ≠ ⊥)
+  : Γ x ≠ ⊥ := λh' => h (w.eq_bot _ h')
 
 theorem FCtx.Wk.support_subset {Γ Δ : FCtx ν α} (w : FCtx.Wk Γ Δ)
   : Δ.support ⊆ Γ.support := by
@@ -97,53 +130,251 @@ instance FCtx.instPartialOrder : PartialOrder (FCtx ν α) where
 
 def FCtx.linf (Δ Δ' : FCtx ν α)
   : FCtx ν α where
-  toFun x := match Δ.toFun x, Δ'.toFun x with
+  toFun x := match Δ x, Δ' x with
     | ⊥, _ | _, ⊥ => ⊥
     | some a, some _ => some a
   support := Δ.support ∩ Δ'.support
   mem_support_toFun := by
     intro x
-    simp only [Finset.mem_inter, mem_support_toFun]
+    simp only [Finset.mem_inter, mem_support]
     split <;> simp [Bot.bot, *]
+
+theorem FCtx.linf_app (Δ Δ' : FCtx ν α) (x : ν)
+  : (FCtx.linf Δ Δ') x = match Δ x, Δ' x with
+    | ⊥, _ | _, ⊥ => ⊥
+    | some a, some _ => some a := by rfl
+
+theorem FCtx.linf_support {Δ Δ' : FCtx ν α}
+  : (FCtx.linf Δ Δ').support = Δ.support ∩ Δ'.support := rfl
+theorem FCtx.linf_mem_support {Δ Δ' : FCtx ν α} (x : ν)
+  : x ∈ (FCtx.linf Δ Δ').support ↔ x ∈ Δ.support ∧ x ∈ Δ'.support := by
+  simp [linf_support]
 
 def FCtx.rinf (Δ Δ' : FCtx ν α)
   : FCtx ν α where
-  toFun x := match Δ.toFun x, Δ'.toFun x with
+  toFun x := match Δ x, Δ' x with
     | ⊥, _ | _, ⊥ => ⊥
     | some _, some a => some a
   support := Δ.support ∩ Δ'.support
   mem_support_toFun := by
     intro x
-    simp only [Finset.mem_inter, mem_support_toFun]
+    simp only [Finset.mem_inter, mem_support]
     split <;> simp [Bot.bot, *]
 
+theorem FCtx.rinf_app (Δ Δ' : FCtx ν α) (x : ν)
+  : (FCtx.rinf Δ Δ') x = match Δ x, Δ' x with
+    | ⊥, _ | _, ⊥ => ⊥
+    | some _, some a => some a := by rfl
+
+theorem FCtx.rinf_support {Δ Δ' : FCtx ν α}
+  : (FCtx.rinf Δ Δ').support = Δ.support ∩ Δ'.support := rfl
+
+theorem FCtx.linf_wk (Δ Δ' : FCtx ν α) : FCtx.Wk Δ (FCtx.linf Δ Δ') := by
+  intro x
+  simp [linf_app]
+  split <;> simp [*]
+
+theorem FCtx.rinf_wk (Δ Δ' : FCtx ν α) : FCtx.Wk Δ' (FCtx.rinf Δ Δ') := by
+  intro x
+  simp [rinf_app]
+  split <;> simp [*]
+
 theorem FCtx.Wk.var_eq {Γ Δ : FCtx ν α} (w : FCtx.Wk Γ Δ) (x : ν) (a b : α)
-  (h : Γ.toFun x = a) (h' : Δ.toFun x = b)
+  (h : Γ x = a) (h' : Δ x = b)
   : a = b := by
   cases w x
   case inl hw => rw [hw] at h'; cases h'
   case inr hw => rw [hw] at h'; rw [h'] at h; cases h; rfl
 
 theorem FCtx.Wk.var {Γ Δ : FCtx ν α} (w : FCtx.Wk Γ Δ) (x : ν) (a : α)
-  (h : Δ.toFun x = a) : Γ.toFun x = a := by
+  (h : Δ x = a) : Γ x = a := by
   cases w x
   case inl hw => rw [hw] at h; cases h
   case inr hw => rw [hw] at h; exact h
 
-def FCtx.Wk.var_eq₂' {Γ Δ Δ' : FCtx ν α} (w : FCtx.Wk Γ Δ) (w' : FCtx.Wk Γ Δ')
-  (x : ν) (a b : α) (h : Δ.toFun x = a) (h' : Δ'.toFun x = b)
+theorem FCtx.Wk.var_eq₂' {Γ Δ Δ' : FCtx ν α} (w : FCtx.Wk Γ Δ) (w' : FCtx.Wk Γ Δ')
+  (x : ν) (a b : α) (h : Δ x = a) (h' : Δ' x = b)
   : (a : WithBot α) = (b : WithBot α) := by rw [<-var w x a h, <-var w' x b h']
 
-def FCtx.Wk.var_eq₂ {Γ Δ Δ' : FCtx ν α} (w : FCtx.Wk Γ Δ) (w' : FCtx.Wk Γ Δ')
-  (x : ν) (a b : α) (h : Δ.toFun x = a) (h' : Δ'.toFun x = b)
+theorem FCtx.Wk.var_eq₂ {Γ Δ Δ' : FCtx ν α} (w : FCtx.Wk Γ Δ) (w' : FCtx.Wk Γ Δ')
+  (x : ν) (a b : α) (h : Δ x = a) (h' : Δ' x = b)
   : a = b := by cases var_eq₂' w w' x a b h h'; rfl
 
-def FCtx.Wk.linf_eq_rinf {Γ Δ Δ' : FCtx ν α} (w : FCtx.Wk Γ Δ) (w' : FCtx.Wk Γ Δ')
+theorem FCtx.Wk.eq_on {Γ Δ : FCtx ν α} (w : FCtx.Wk Γ Δ)
+  : ∀x ∈ Δ.support, Δ x = Γ x := by
+  intro x hx
+  cases w x with
+  | inl h => rw [mem_support] at hx; exact (hx h).elim
+  | inr h => exact h
+
+theorem FCtx.Wk.linf_eq_rinf {Γ Δ Δ' : FCtx ν α} (w : FCtx.Wk Γ Δ) (w' : FCtx.Wk Γ Δ')
   : FCtx.linf Δ Δ' = FCtx.rinf Δ Δ' := by
   apply FCtx.ext
-  funext x
-  simp only [linf, rinf]
+  intro x
+  simp only [DFunLike.coe, linf, rinf]
   split
   . rfl
   . rfl
   . apply var_eq₂' w w' <;> assumption
+
+theorem FCtx.Wk.linf_wk_left {Γ Δ Δ' : FCtx ν α} (_ : FCtx.Wk Γ Δ) (_ : FCtx.Wk Γ Δ')
+  : FCtx.Wk Δ (FCtx.linf Δ Δ') := linf_wk Δ Δ'
+theorem FCtx.Wk.linf_wk_right {Γ Δ Δ' : FCtx ν α} (w : FCtx.Wk Γ Δ) (w' : FCtx.Wk Γ Δ')
+  : FCtx.Wk Δ' (FCtx.linf Δ Δ') := linf_eq_rinf w w' ▸ rinf_wk Δ Δ'
+
+theorem FCtx.Wk.rinf_wk_left {Γ Δ Δ' : FCtx ν α} (w : FCtx.Wk Γ Δ) (w' : FCtx.Wk Γ Δ')
+  : FCtx.Wk Δ (FCtx.rinf Δ Δ') := linf_eq_rinf w w' ▸ linf_wk Δ Δ'
+theorem FCtx.Wk.rinf_wk_right {Γ Δ Δ' : FCtx ν α} (_ : FCtx.Wk Γ Δ) (_ : FCtx.Wk Γ Δ')
+  : FCtx.Wk Δ' (FCtx.rinf Δ Δ') := rinf_wk Δ Δ'
+
+theorem FCtx.linf_eq_none_left {Δ Δ' : FCtx ν α} (x : ν) (h : Δ x = ⊥)
+  : FCtx.linf Δ Δ' x = ⊥ := by
+  simp only [linf_app]
+  split <;> simp only [h] at *
+theorem FCtx.linf_eq_none_right {Δ Δ' : FCtx ν α} (x : ν) (h : Δ' x = ⊥)
+  : FCtx.linf Δ Δ' x = ⊥ := by
+  simp only [linf_app] at *
+  split <;> simp only [h] at *
+theorem FCtx.linf_eq_none_or {Δ Δ' : FCtx ν α} (x : ν) (h : FCtx.linf Δ Δ' x = ⊥)
+  : Δ x = ⊥ ∨ Δ' x = ⊥ := by
+  simp only [linf_app] at h
+  rw [<-h] -- hack until term-to-split is supported...
+  split <;> simp [*, Bot.bot]
+theorem FCtx.linf_eq_none_iff {Δ Δ' : FCtx ν α} (x : ν)
+  : FCtx.linf Δ Δ' x = ⊥ ↔ Δ x = ⊥ ∨ Δ' x = ⊥ :=
+  ⟨linf_eq_none_or x, λh => h.elim (linf_eq_none_left x) (linf_eq_none_right x)⟩
+
+theorem FCtx.linf_var_left {Δ Δ' : FCtx ν α} (x : ν) (a : α)
+  : FCtx.linf Δ Δ' x = a → Δ x = a := by
+  simp only [linf_app]
+  split
+  . intro h; cases h
+  . intro h; cases h
+  . intro h; rw [<-h]; assumption
+theorem FCtx.linf_var_right {Δ Δ' : FCtx ν α} (x : ν) (a : α)
+  : FCtx.linf Δ Δ' x = a → ∃b : α, Δ' x = b := by
+  simp only [linf_app]
+  split
+  . intro h; cases h
+  . intro h; cases h
+  . intro _; constructor; assumption
+
+theorem FCtx.linf_var_left_eq' {Δ Δ' : FCtx ν α} (x : ν) (a : α) (bb : WithBot α)
+  (h : FCtx.linf Δ Δ' x = a) (h' : Δ x = bb) : a = bb := by
+    rw [<-linf_var_left x a h]; assumption
+theorem FCtx.linf_var_left_eq {Δ Δ' : FCtx ν α} (x : ν) (a b : α)
+  (h : FCtx.linf Δ Δ' x = a) (h' : Δ x = b) : a = b := by
+    cases linf_var_left_eq' x a b h h'; rfl
+
+theorem FCtx.linf_support_eq_left {Δ Δ' : FCtx ν α} (x : ν)
+  (h : x ∈ (linf Δ Δ').support) : FCtx.linf Δ Δ' x = Δ x := (linf_wk Δ Δ').eq_on x h
+
+theorem FCtx.linf_var_eq_left {Δ Δ' : FCtx ν α} (x : ν) (a : α)
+  (h : FCtx.linf Δ Δ' x = a)
+  : FCtx.linf Δ Δ' x = Δ x := by
+    rw [h]
+    apply Eq.symm
+    apply linf_var_left
+    exact h
+theorem FCtx.linf_right_var_eq_left {Δ Δ' : FCtx ν α} (x : ν) (a : α)
+  (h : Δ' x = a)
+  : FCtx.linf Δ Δ' x = Δ x := by
+    rw [linf_app]
+    split
+    . simp [*, Bot.bot] at *
+    . rw [h] at *; contradiction
+    . simp [*]
+
+theorem FCtx.linf_some_eq_left {Δ Δ' : FCtx ν α} (x : ν)
+: (∃a : α, FCtx.linf Δ Δ' x = a) → FCtx.linf Δ Δ' x = Δ x := by
+  intro ⟨a, h⟩
+  rw [h]
+  apply Eq.symm
+  apply linf_var_left
+  exact h
+theorem FCtx.linf_right_some_eq_left {Δ Δ' : FCtx ν α} (x : ν)
+  : (∃a: α, Δ' x = a) → FCtx.linf Δ Δ' x = Δ x := by
+  intro ⟨a, h⟩
+  apply linf_right_var_eq_left _ _ h
+theorem FCtx.linf_right_support_eq_left {Δ Δ' : FCtx ν α} (x : ν)
+  (h : x ∈ Δ'.support) : FCtx.linf Δ Δ' x = Δ x := by
+  apply linf_right_some_eq_left _ ((mem_support_exists _).mp h)
+  rfl
+
+theorem FCtx.linf_assoc (Δ₁ Δ₂ Δ₃ : FCtx ν α)
+  : FCtx.linf (FCtx.linf Δ₁ Δ₂) Δ₃ = FCtx.linf Δ₁ (FCtx.linf Δ₂ Δ₃) := by
+  apply FCtx.ext
+  intro x
+  conv =>
+    rhs
+    rw [linf_app]
+  split
+  . apply linf_eq_none_left; apply linf_eq_none_left; assumption
+  . simp only [linf_eq_none_iff]
+    rw [or_assoc]
+    apply Or.inr
+    apply linf_eq_none_or
+    assumption
+  . rename_i h
+    rw [linf_right_some_eq_left _ (linf_var_right _ _ h)]
+    rw [linf_right_var_eq_left _ _ (linf_var_left _ _ h)]
+    assumption
+
+theorem FCtx.linf_comm (Δ Δ' : FCtx ν α)
+  : FCtx.linf Δ Δ' = FCtx.rinf Δ' Δ := by
+  apply FCtx.ext
+  intro x;
+  simp only [linf_app, rinf_app]
+  split
+  . split
+    . rfl
+    . rfl
+    . simp [*] at *
+  . split
+    . rfl
+    . rfl
+    . simp [*] at *
+  . split
+    . simp [*] at *
+    . simp [*] at *
+    . rename_i h _ _ _ _ _ _ h'
+      rw [<-h, <-h']
+
+theorem FCtx.rinf_comm (Δ Δ' : FCtx ν α)
+  : FCtx.rinf Δ Δ' = FCtx.linf Δ' Δ := by
+  rw [linf_comm]
+
+--TODO: rinf_assoc, etc...
+
+def FCtx.lsup (Δ Δ' : FCtx ν α)
+  : FCtx ν α where
+  toFun x := match Δ x, Δ' x with
+    | ⊥, _ => Δ' x
+    | _, ⊥ => Δ x
+    | some a, some _ => some a
+  support := Δ.support ∪ Δ'.support
+  mem_support_toFun := by
+    intro x
+    simp only [Finset.mem_union, mem_support]
+    split <;> simp [Bot.bot, *]
+
+def FCtx.rsup (Δ Δ' : FCtx ν α)
+  : FCtx ν α where
+  toFun x := match Δ x, Δ' x with
+    | ⊥, _ => Δ' x
+    | _, ⊥ => Δ x
+    | some _, some a => some a
+  support := Δ.support ∪ Δ'.support
+  mem_support_toFun := by
+    intro x
+    simp only [Finset.mem_union, mem_support]
+    split <;> simp [Bot.bot, *]
+
+--TODO: wk lemmas, assoc, etc...
+
+structure FLCtx (κ : Type _) (ν : Type _) (α : Type _) : Type _ where
+  toFun : κ → WithBot (FCtx ν α)
+  support : Finset κ
+  mem_support_toFun : ∀x, x ∈ support ↔ toFun x ≠ ⊥
+
+--TODO: FLCtx.linf, rinf, lsup, rsup, and lemmata
